testcases/printtest/exec_IR.ll
@@ -1,27 +1,35 @@
-; ModuleID = '/home/clexma/Desktop/Disk_D/Tools/SMACK/smack/build/b-zlu73utw.bc'
+; ModuleID = '/home/clexma/Desktop/Disk_D/Tools/SMACK/smack/build/b-frra87f7.bc'
 source_filename = "llvm-link"
 target datalayout = "e-m:e-p270:32:32-p271:32:32-p272:64:64-i64:64-f80:128-n8:16:32:64-S128"
 target triple = "x86_64-pc-linux-gnu"
 
-%struct.test = type { i32, i8, %struct.test* }
+%struct.TData = type { i8*, i8* }
 
 ; Function Attrs: noinline nounwind uwtable
 define dso_local i32 @main() #0 !dbg !7 {
-  %1 = alloca %struct.test, align 8, !verifier.code !11
-  call void @llvm.dbg.declare(metadata %struct.test* %1, metadata !12, metadata !DIExpression()), !dbg !21, !verifier.code !11
-  %2 = getelementptr inbounds %struct.test, %struct.test* %1, i32 0, i32 0, !dbg !22, !verifier.code !11
-  store i32 0, i32* %2, align 8, !dbg !23, !verifier.code !11
-  %3 = getelementptr inbounds %struct.test, %struct.test* %1, i32 0, i32 1, !dbg !24, !verifier.code !11
-  store i8 100, i8* %3, align 4, !dbg !25, !verifier.code !11
-  %4 = getelementptr inbounds %struct.test, %struct.test* %1, i32 0, i32 1, !dbg !26, !verifier.code !11
-  %5 = load i8, i8* %4, align 4, !dbg !26, !verifier.code !11
-  %6 = sext i8 %5 to i32, !dbg !27, !verifier.code !11
-  call void @llvm.dbg.value(metadata i32 %6, metadata !28, metadata !DIExpression()), !dbg !29, !verifier.code !11
-  ret i32 0, !dbg !30, !verifier.code !11
+  %1 = alloca %struct.TData, align 8, !verifier.code !11
+  call void @llvm.dbg.declare(metadata %struct.TData* %1, metadata !12, metadata !DIExpression()), !dbg !19, !verifier.code !11
+  call void @llvm.dbg.value(metadata %struct.TData* %1, metadata !20, metadata !DIExpression()), !dbg !22, !verifier.code !11
+  %2 = call noalias i8* @malloc(i64 16) #3, !dbg !23, !verifier.code !11
+  %3 = getelementptr inbounds %struct.TData, %struct.TData* %1, i32 0, i32 0, !dbg !24, !verifier.code !11
+  store i8* %2, i8** %3, align 8, !dbg !25, !verifier.code !11
+  %4 = call noalias i8* @malloc(i64 24) #3, !dbg !26, !verifier.code !11
+  %5 = getelementptr inbounds %struct.TData, %struct.TData* %1, i32 0, i32 1, !dbg !27, !verifier.code !11
+  store i8* %4, i8** %5, align 8, !dbg !28, !verifier.code !11
+  %6 = getelementptr inbounds %struct.TData, %struct.TData* %1, i32 0, i32 0, !dbg !29, !verifier.code !11
+  %7 = load i8*, i8** %6, align 8, !dbg !29, !verifier.code !11
+  call void @llvm.dbg.value(metadata i8* %7, metadata !30, metadata !DIExpression()), !dbg !22, !verifier.code !11
+  %8 = getelementptr inbounds %struct.TData, %struct.TData* %1, i32 0, i32 1, !dbg !31, !verifier.code !11
+  %9 = load i8*, i8** %8, align 8, !dbg !31, !verifier.code !11
+  call void @llvm.dbg.value(metadata i8* %9, metadata !32, metadata !DIExpression()), !dbg !22, !verifier.code !11
+  ret i32 0, !dbg !33, !verifier.code !11
 }
 
 ; Function Attrs: nounwind readnone speculatable willreturn
 declare void @llvm.dbg.declare(metadata, metadata, metadata) #1
+
+; Function Attrs: nounwind
+declare dso_local noalias i8* @malloc(i64) #2
 
 ; Function Attrs: nounwind readnone speculatable willreturn
 declare void @llvm.dbg.value(metadata, metadata, metadata) #1
@@ -33,6 +41,8 @@ entry:
 
 attributes #0 = { noinline nounwind uwtable "correctly-rounded-divide-sqrt-fp-math"="false" "disable-tail-calls"="false" "frame-pointer"="all" "less-precise-fpmad"="false" "min-legal-vector-width"="0" "no-infs-fp-math"="false" "no-jump-tables"="false" "no-nans-fp-math"="false" "no-signed-zeros-fp-math"="false" "no-trapping-math"="false" "stack-protector-buffer-size"="8" "target-cpu"="x86-64" "target-features"="+cx8,+fxsr,+mmx,+sse,+sse2,+x87" "unsafe-fp-math"="false" "use-soft-float"="false" }
 attributes #1 = { nounwind readnone speculatable willreturn }
+attributes #2 = { nounwind "correctly-rounded-divide-sqrt-fp-math"="false" "disable-tail-calls"="false" "frame-pointer"="all" "less-precise-fpmad"="false" "no-infs-fp-math"="false" "no-nans-fp-math"="false" "no-signed-zeros-fp-math"="false" "no-trapping-math"="false" "stack-protector-buffer-size"="8" "target-cpu"="x86-64" "target-features"="+cx8,+fxsr,+mmx,+sse,+sse2,+x87" "unsafe-fp-math"="false" "use-soft-float"="false" }
+attributes #3 = { nounwind }
 
 !llvm.dbg.cu = !{!0}
 !llvm.ident = !{!3}
@@ -50,22 +60,25 @@ attributes #1 = { nounwind readnone speculatable willreturn }
 !9 = !{!10}
 !10 = !DIBasicType(name: "int", size: 32, encoding: DW_ATE_signed)
 !11 = !{i1 false}
-!12 = !DILocalVariable(name: "i", scope: !7, file: !1, line: 35, type: !13)
-!13 = !DIDerivedType(tag: DW_TAG_typedef, name: "test_type", file: !1, line: 8, baseType: !14)
-!14 = distinct !DICompositeType(tag: DW_TAG_structure_type, name: "test", file: !1, line: 4, size: 128, elements: !15)
-!15 = !{!16, !17, !19}
-!16 = !DIDerivedType(tag: DW_TAG_member, name: "a", scope: !14, file: !1, line: 5, baseType: !10, size: 32)
-!17 = !DIDerivedType(tag: DW_TAG_member, name: "b", scope: !14, file: !1, line: 6, baseType: !18, size: 8, offset: 32)
-!18 = !DIBasicType(name: "char", size: 8, encoding: DW_ATE_signed_char)
-!19 = !DIDerivedType(tag: DW_TAG_member, name: "next", scope: !14, file: !1, line: 7, baseType: !20, size: 64, offset: 64)
-!20 = !DIDerivedType(tag: DW_TAG_pointer_type, baseType: !14, size: 64)
-!21 = !DILocation(line: 35, column: 15, scope: !7)
-!22 = !DILocation(line: 36, column: 7, scope: !7)
-!23 = !DILocation(line: 36, column: 9, scope: !7)
-!24 = !DILocation(line: 37, column: 7, scope: !7)
-!25 = !DILocation(line: 37, column: 9, scope: !7)
-!26 = !DILocation(line: 38, column: 15, scope: !7)
-!27 = !DILocation(line: 38, column: 13, scope: !7)
-!28 = !DILocalVariable(name: "a", scope: !7, file: !1, line: 38, type: !10)
-!29 = !DILocation(line: 0, scope: !7)
-!30 = !DILocation(line: 46, column: 1, scope: !7)
+!12 = !DILocalVariable(name: "data", scope: !7, file: !1, line: 23, type: !13)
+!13 = !DIDerivedType(tag: DW_TAG_typedef, name: "TData", file: !1, line: 13, baseType: !14)
+!14 = distinct !DICompositeType(tag: DW_TAG_structure_type, file: !1, line: 10, size: 128, elements: !15)
+!15 = !{!16, !18}
+!16 = !DIDerivedType(tag: DW_TAG_member, name: "lo", scope: !14, file: !1, line: 11, baseType: !17, size: 64)
+!17 = !DIDerivedType(tag: DW_TAG_pointer_type, baseType: null, size: 64)
+!18 = !DIDerivedType(tag: DW_TAG_member, name: "hi", scope: !14, file: !1, line: 12, baseType: !17, size: 64, offset: 64)
+!19 = !DILocation(line: 23, column: 11, scope: !7)
+!20 = !DILocalVariable(name: "pdata", scope: !7, file: !1, line: 24, type: !21)
+!21 = !DIDerivedType(tag: DW_TAG_pointer_type, baseType: !13, size: 64)
+!22 = !DILocation(line: 0, scope: !7)
+!23 = !DILocation(line: 27, column: 17, scope: !7)
+!24 = !DILocation(line: 27, column: 12, scope: !7)
+!25 = !DILocation(line: 27, column: 15, scope: !7)
+!26 = !DILocation(line: 28, column: 17, scope: !7)
+!27 = !DILocation(line: 28, column: 12, scope: !7)
+!28 = !DILocation(line: 28, column: 15, scope: !7)
+!29 = !DILocation(line: 29, column: 23, scope: !7)
+!30 = !DILocalVariable(name: "lo", scope: !7, file: !1, line: 29, type: !17)
+!31 = !DILocation(line: 30, column: 23, scope: !7)
+!32 = !DILocalVariable(name: "hi", scope: !7, file: !1, line: 30, type: !17)
+!33 = !DILocation(line: 46, column: 1, scope: !7)
